src/HOL/MicroJava/J/JTypeSafe.thy
@@ -206,7 +206,7 @@ apply( unfold c_hupd_def)
 apply( simp_all)
 apply( tactic "ALLGOALS strip_tac")
 apply( tactic {* ALLGOALS (eresolve_tac [thm "ty_expr.cases", thm "ty_exprs.cases", thm "wt_stmt.cases"]
-                 THEN_ALL_NEW Full_simp_tac) *})
+                 THEN_ALL_NEW (full_simp_tac (simpset_of @{theory Conform}))) *})
 apply(tactic "ALLGOALS (EVERY' [REPEAT o (etac conjE), REPEAT o hyp_subst_tac])")
 
 -- "Level 7"
@@ -246,10 +246,11 @@ apply( fast elim: conforms_localD [THEN lconfD])
 
 -- "for FAss"
 apply( tactic {* EVERY'[eresolve_tac [thm "ty_expr.cases", thm "ty_exprs.cases", thm "wt_stmt.cases"] 
-       THEN_ALL_NEW Full_simp_tac, REPEAT o (etac conjE), hyp_subst_tac] 3*})
+       THEN_ALL_NEW (full_simp_tac @{simpset}), REPEAT o (etac conjE), hyp_subst_tac] 3*})
 
 -- "for if"
-apply( tactic {* (case_tac "the_Bool v" THEN_ALL_NEW Asm_full_simp_tac) 7*})
+apply( tactic {* (case_tac "the_Bool v" THEN_ALL_NEW
+  (asm_full_simp_tac @{simpset})) 7*})
 
 apply (tactic "forward_hyp_tac")
 
@@ -281,7 +282,7 @@ apply (rule conjI)
 -- "7 LAss"
 apply (fold fun_upd_def)
 apply( tactic {* (eresolve_tac [thm "ty_expr.cases", thm "ty_exprs.cases", thm "wt_stmt.cases"] 
-                 THEN_ALL_NEW Full_simp_tac) 1 *})
+                 THEN_ALL_NEW (full_simp_tac @{simpset})) 1 *})
 apply (intro strip)
 apply (case_tac E)
 apply (simp)
